Removed alg_compile, moved correctness into compiler

Compiler.thy
@@ -9,198 +9,172 @@ abbreviation code_compile :: "ty expr\<^sub>s \<Rightarrow> mach list" where
 abbreviation compile :: "unit expr\<^sub>s \<rightharpoonup> mach list \<times> ty" where 
   "compile \<equiv> map_option (apfst code_compile) \<circ> typecheck"
 
-primrec quick_convert :: "var set \<Rightarrow> unit expr\<^sub>s \<Rightarrow> uterm expr\<^sub>s \<times> var set" where
-  "quick_convert vs (Var\<^sub>s x) = (Var\<^sub>s x, {})"
-| "quick_convert vs (Const\<^sub>s k) = (Const\<^sub>s k, {})"
-| "quick_convert vs (Lam\<^sub>s x t e) = (
-    let v = fresh vs
-    in let (e', vs') = quick_convert (insert v vs) e
-    in (Lam\<^sub>s x (Var v) e', insert v vs'))"
-| "quick_convert vs (App\<^sub>s e\<^sub>1 e\<^sub>2) = (
-    let v = fresh vs
-    in let (e\<^sub>1', vs') = quick_convert (insert v vs) e\<^sub>1 
-    in let (e\<^sub>2', vs'') = quick_convert (insert v (vs \<union> vs')) e\<^sub>2 
-    in (App\<^sub>s e\<^sub>1' e\<^sub>2', insert v (vs' \<union> vs'')))"
-| "quick_convert vs (Let\<^sub>s x e\<^sub>1 e\<^sub>2) = (
-    let (e\<^sub>1', vs') = quick_convert vs e\<^sub>1 
-    in let (e\<^sub>2', vs'') = quick_convert (vs \<union> vs') e\<^sub>2 
-    in (Let\<^sub>s x e\<^sub>1' e\<^sub>2', (vs' \<union> vs'')))"
+abbreviation initial_state :: "mach list \<Rightarrow> mach_state" where
+  "initial_state cd \<equiv> MS (case_reg 0 1 2 11 0) ((\<lambda>x. 0)(7 := 1)) (length cd)"
 
-primrec collect_constraints :: "subst \<Rightarrow> var set \<Rightarrow> unit expr\<^sub>s \<Rightarrow> uterm \<times> var set \<times> constraint" where
-  "collect_constraints \<Gamma> vs (Var\<^sub>s x) = (case \<Gamma> x of 
-      Some t \<Rightarrow> (t, {}, []) 
-    | None \<Rightarrow> (Num\<^sub>\<tau>, {}, fail))"
-| "collect_constraints \<Gamma> vs (Const\<^sub>s k) = (Num\<^sub>\<tau>, {}, [])"
-| "collect_constraints \<Gamma> vs (Lam\<^sub>s x u e) = (
-    let v = fresh vs
-    in let (t, vs', con) = collect_constraints (\<Gamma>(x \<mapsto> Var v)) (insert v vs) e
-    in (Arrow\<^sub>\<tau> (Var v) t, insert v vs', con))"
-| "collect_constraints \<Gamma> vs (App\<^sub>s e\<^sub>1 e\<^sub>2) = (
-    let v = fresh vs
-    in let (t\<^sub>1, vs', con\<^sub>1) = collect_constraints \<Gamma> (insert v vs) e\<^sub>1 
-    in let (t\<^sub>2, vs'', con\<^sub>2) = collect_constraints \<Gamma> (insert v (vs \<union> vs')) e\<^sub>2 
-    in (Var v, insert v (vs' \<union> vs''), con\<^sub>1 @ con\<^sub>2 @ [(t\<^sub>1, Arrow\<^sub>\<tau> t\<^sub>2 (Var v))]))"
-| "collect_constraints \<Gamma> vs (Let\<^sub>s x e\<^sub>1 e\<^sub>2) = (
-    let (t\<^sub>1, vs', con\<^sub>1) = collect_constraints \<Gamma> vs e\<^sub>1 
-    in let (t\<^sub>2, vs'', con\<^sub>2) = collect_constraints \<Gamma> (vs \<union> vs') e\<^sub>2 
-    in (t\<^sub>2, (vs' \<union> vs''), con\<^sub>1 @ con\<^sub>2))"
+primrec final_state :: "mach_state \<Rightarrow> bool" where
+  "final_state (MS rs mem pc) = (pc = 0 \<and> rs R3 = 6 \<and> rs R4 = 3)"
 
-fun tree_code_size :: "code\<^sub>e \<Rightarrow> nat"
-and tree_code_size_list :: "code\<^sub>e list \<Rightarrow> nat" where
-  "tree_code_size (Lookup\<^sub>e x) = 0"
-| "tree_code_size (PushCon\<^sub>e k) = 0"
-| "tree_code_size (PushLam\<^sub>e cd) = tree_code_size_list cd"
-| "tree_code_size Apply\<^sub>e = 0"
-| "tree_code_size PushEnv\<^sub>e = 0"
-| "tree_code_size PopEnv\<^sub>e = 0"
-| "tree_code_size Return\<^sub>e = 0"
-| "tree_code_size Jump\<^sub>e = 0"
-| "tree_code_size_list [] = 0"
-| "tree_code_size_list (Apply\<^sub>e # Return\<^sub>e # cd) = Suc (tree_code_size_list cd)"
-| "tree_code_size_list (op # cd) = Suc (tree_code_size op + tree_code_size_list cd)"
-
-lemma [simp]: "op \<noteq> Return\<^sub>e \<Longrightarrow> tree_code_size_list (op # cd) < tree_code_size_list (Apply\<^sub>e # op # cd)"
-  by (cases op) simp_all
-
-primrec alg_compile1 :: "var list \<Rightarrow> unit expr\<^sub>s \<Rightarrow> code\<^sub>e list \<Rightarrow> code\<^sub>e list" where
-  "alg_compile1 \<Phi> (Var\<^sub>s x) acc = Lookup\<^sub>e (the (idx_of \<Phi> x)) # acc"
-| "alg_compile1 \<Phi> (Const\<^sub>s k) acc = PushCon\<^sub>e k # acc"
-| "alg_compile1 \<Phi> (Lam\<^sub>s x u e) acc = PushLam\<^sub>e (alg_compile1 (insert_at 0 x \<Phi>) e [Return\<^sub>e]) # acc"
-| "alg_compile1 \<Phi> (App\<^sub>s e\<^sub>1 e\<^sub>2) acc = alg_compile1 \<Phi> e\<^sub>1 (alg_compile1 \<Phi> e\<^sub>2 (Apply\<^sub>e # acc))"
-| "alg_compile1 \<Phi> (Let\<^sub>s x e\<^sub>1 e\<^sub>2) acc = 
-    alg_compile1 \<Phi> e\<^sub>1 (PushEnv\<^sub>e # alg_compile1 (insert_at 0 x \<Phi>) e\<^sub>2 (PopEnv\<^sub>e # acc))"
-
-function alg_compile2 :: "nat \<Rightarrow> code\<^sub>e list \<Rightarrow> code\<^sub>b list \<Rightarrow> code\<^sub>b list" where
-  "alg_compile2 lib [] acc = acc"
-| "alg_compile2 lib (Lookup\<^sub>e x # cd) acc = alg_compile2 lib cd (Lookup\<^sub>b x # acc)"
-| "alg_compile2 lib (PushCon\<^sub>e k # cd) acc = alg_compile2 lib cd (PushCon\<^sub>b k # acc)"
-| "alg_compile2 lib (PushLam\<^sub>e cd' # cd) acc =
-    alg_compile2 lib cd' 
-      (alg_compile2 (lib + tree_code_size_list cd') cd 
-        (PushLam\<^sub>b (lib + tree_code_size_list cd') # acc))"
-| "alg_compile2 lib (Apply\<^sub>e # []) acc = Apply\<^sub>b # acc"
-| "alg_compile2 lib (Apply\<^sub>e # op # cd) acc = (
-    if op = Return\<^sub>e 
-    then alg_compile2 lib cd (Jump\<^sub>b # acc)
-    else alg_compile2 lib (op # cd) (Apply\<^sub>b # acc))"
-| "alg_compile2 lib (PushEnv\<^sub>e # cd) acc = alg_compile2 lib cd (PushEnv\<^sub>b # acc)"
-| "alg_compile2 lib (PopEnv\<^sub>e # cd) acc = alg_compile2 lib cd acc"
-| "alg_compile2 lib (Return\<^sub>e # cd) acc = alg_compile2 lib cd (Return\<^sub>b # acc)"
-| "alg_compile2 lib (Jump\<^sub>e # cd) acc = alg_compile2 lib cd (Jump\<^sub>b # acc)"
-  by pat_completeness auto
-termination
-  by (relation "measure (tree_code_size_list \<circ> fst \<circ> snd)") simp_all
-
-fun assembly_mapb :: "code\<^sub>b list \<Rightarrow> nat \<Rightarrow> nat" where
-  "assembly_mapb [] x = 0"
-| "assembly_mapb (op # cd) 0 = 0"
-| "assembly_mapb (Lookup\<^sub>b k # cd) (Suc x) = 8 + 2 * k + assembly_mapb cd x"
-| "assembly_mapb (PushCon\<^sub>b k # cd) (Suc x) = 6 + assembly_mapb cd x"
-| "assembly_mapb (PushLam\<^sub>b pc # cd) (Suc x) = 10 + assembly_mapb cd x"
-| "assembly_mapb (Apply\<^sub>b # cd) (Suc x) = 21 + assembly_mapb cd x"
-| "assembly_mapb (PushEnv\<^sub>b # cd) (Suc x) = 14 + assembly_mapb cd x"
-| "assembly_mapb (Return\<^sub>b # cd) (Suc x) = 6 + assembly_mapb cd x"
-| "assembly_mapb (Jump\<^sub>b # cd) (Suc x) = 20 + assembly_mapb cd x"
-
-fun alg_assemble :: "(nat \<Rightarrow> nat) \<Rightarrow> nat \<Rightarrow> code\<^sub>b list \<Rightarrow> mach list" where
-  "alg_assemble mp ix [] = []"
-| "alg_assemble mp ix (Lookup\<^sub>b x # cd) = 
-    [LODI R5 0, ADDI R3 4, STO R3 R5, LOD R5 R5, SUBI R5 8] @ 
-      concat (replicate x [LOD R5 R5, SUBI R5 4]) @ 
-      [LOD R5 R5, SUBI R5 4, MOV R5 R4] @ 
-      alg_assemble mp (Suc ix) cd"
-| "alg_assemble mp ix (PushCon\<^sub>b k # cd) = 
-    [ADDI R1 4, STOI R1 0, ADDI R1 4, STOI R1 k, ADDI R3 4, STO R3 R1] @ 
-      alg_assemble mp (Suc ix) cd"
-| "alg_assemble mp ix (PushLam\<^sub>b pc # cd) = 
-    [ADDI R1 4, STOI R1 (mp pc), LODI R5 0, ADDI R1 4, 
-      STO R1 R5, LOD R5 R5, SUBI R5 4, MOV R5 R4, ADDI R3 4, STO R3 R1] @ 
-      alg_assemble mp (Suc ix) cd"
-| "alg_assemble mp ix (Apply\<^sub>b # cd) = 
-    [JMP R5, LOD R5 R5, ADDI R5 4, STOI R3 0, LOD R5 R3, ADDI R2 4, STO R2 R5, LOD R5 R5, LOD R5 R3, 
-      SUBI R3 4, ADDI R4 4, STO R4 R5, ADDI R5 4, MOV R5 R2, ADDI R4 4, STOI R4 (mp ix), ADDI R2 4, 
-      STO R2 R5, STOI R3 0, LOD R5 R3, SUBI R3 4] @ 
-      alg_assemble mp (Suc ix) cd"
-| "alg_assemble mp ix (PushEnv\<^sub>b # cd) = 
-    [LODI R5 0, ADDI R4 4, STO R4 R5, SUBI R5 8, MOV R5 R2, ADDI R2 4, STO R2 R5, LOD R5 R4, 
-      SUBI R4 4, ADDI R2 4, STO R2 R5, STOI R3 0, LOD R5 R3, SUBI R3 4] @ 
-      alg_assemble mp (Suc ix) cd"
-| "alg_assemble mp ix (Return\<^sub>b # cd) = 
-    [JMP R5, STOI R4 0, LOD R5 R4, SUBI R4 4, STOI R4 0, SUBI R4 4] @ 
-      alg_assemble mp (Suc ix) cd"
-| "alg_assemble mp ix (Jump\<^sub>b # cd) = 
-    [JMP R5, LOD R5 R5, ADDI R5 4, STOI R3 0, LOD R5 R3, ADDI R2 4, STO R2 R5, LOD R5 R5, LOD R5 R3, 
-      SUBI R3 4, ADDI R4 4, STO R4 R5, SUBI R4 4, ADDI R5 4, MOV R5 R2, ADDI R2 4, STO R2 R5, 
-      STOI R3 0, LOD R5 R3, SUBI R3 4] @ 
-      alg_assemble mp (Suc ix) cd"
-
-definition alg_compile3 :: "code\<^sub>b list \<Rightarrow> mach list" where
-  "alg_compile3 cd = alg_assemble (assembly_mapb cd) 0 cd"
-
-definition alg_compile :: "unit expr\<^sub>s \<rightharpoonup> mach list \<times> ty" where
-  "alg_compile e = (
-    let (t, vs, con) = collect_constraints Map.empty {} e
-    in case unify con of
-        None \<Rightarrow> None
-      | Some s \<Rightarrow> Some (alg_compile3 (alg_compile2 0 (alg_compile1 [] e [] @ [Return\<^sub>e]) []), 
-                        to_type (subst s t)))"
-
-lemma [simp]: "encode' (unname' \<Phi> (map_expr\<^sub>s to_type (map_expr\<^sub>s (subst sub) e))) = 
-    encode' (unname' \<Phi> (map_expr\<^sub>s to_type e))"
-  by (induction e arbitrary: \<Phi>) simp_all
-
-lemma [simp]: "encode' \<circ> unname \<circ> map_expr\<^sub>s to_type \<circ> map_expr\<^sub>s (subst sub) = 
-    encode' \<circ> unname \<circ> map_expr\<^sub>s to_type"
-  by (auto simp add: unname_def)
-
-lemma [simp]: "typecheck' \<Gamma> vs e = (e', t, vs', con) \<Longrightarrow> quick_convert vs e = (e', vs')"
-  by (induction e arbitrary: \<Gamma> vs e' t vs' con) 
-     (simp_all add: Let_def split: option.splits prod.splits)
-
-lemma [simp]: "quick_convert vs e = (e', vs') \<Longrightarrow> 
-    alg_compile1 \<Phi> e acc = encode' (unname' \<Phi> (map_expr\<^sub>s to_type e')) @ acc"
-  by (induction e arbitrary: \<Phi> acc vs e' vs') (auto simp add: Let_def split: prod.splits)
-
-lemma [simp]: "typecheck' \<Gamma> vs e = (e', t, vs', con) \<Longrightarrow> 
-  alg_compile1 \<Phi> e acc = encode' (unname' \<Phi> (map_expr\<^sub>s to_type e')) @ acc"
+theorem tc_failure: "compile e = None \<Longrightarrow> 
+  \<nexists>e\<^sub>t t. (Map.empty \<turnstile>\<^sub>t e\<^sub>t : t) \<and> e = erase e\<^sub>t"
 proof -
-  assume "typecheck' \<Gamma> vs e = (e', t, vs', con)"
-  hence "quick_convert vs e = (e', vs')" by simp
-  thus ?thesis by simp
+  assume "compile e = None"
+  hence "typecheck e = None" by (auto split: option.splits prod.splits)
+  thus ?thesis by (metis typecheck_fails)
 qed
 
-lemma [simp]: "tree_code_size_list cd = code_list_size (tco_code cd)"
-  by (induction cd rule: tco_code.induct) (simp_all split: list.splits)
+lemma [simp]: "properly_terminated\<^sub>e (cd @ [Apply\<^sub>e, Return\<^sub>e]) = properly_terminated\<^sub>e (cd @ [Return\<^sub>e])"
+  by (induction cd rule: properly_terminated\<^sub>e.induct) simp_all
 
-lemma [simp]: "alg_compile2 lib cd acc = flatten_code' lib (tco_code cd) @ acc"
-proof (induction lib cd acc rule: alg_compile2.induct)
-  case (4 lib cd' cd acc)
-  then show ?case by simp
-next
-  case (6 lib op cd acc)
-  thus ?case by (induction op) simp_all
-next
-  case (8 lib cd acc)
-  then show ?case by simp
-qed simp_all
+lemma [simp]: "properly_terminated\<^sub>e (e1 @ [Return\<^sub>e]) \<Longrightarrow> properly_terminated\<^sub>e (e2 @ [Return\<^sub>e]) \<Longrightarrow> 
+    properly_terminated\<^sub>e (e1 @ e2 @ [Apply\<^sub>e, Return\<^sub>e])"
+  by (induction e1 rule: properly_terminated\<^sub>e.induct) simp_all
 
-lemma alg_assemble_simp [simp]: "alg_assemble mp ix cd = 
-    disassemble (concat (map_with_idx (\<lambda>x. assemble_op mp (ix + x)) cd))"
-  by (induction mp ix cd rule: alg_assemble.induct) (simp_all add: disassemble_def)
+lemma [simp]: "properly_terminated\<^sub>e (cd @ [Return\<^sub>e]) \<Longrightarrow> 
+    properly_terminated\<^sub>e (cd @ [PopEnv\<^sub>e, Return\<^sub>e])"
+  by (induction cd rule: properly_terminated\<^sub>e.induct) simp_all
 
-lemma [simp]: "assembly_mapb cd x = assembly_map cd x"
-  by (induction cd x rule: assembly_mapb.induct) simp_all
+lemma [simp]: "properly_terminated\<^sub>e (e1 @ [Return\<^sub>e]) \<Longrightarrow> properly_terminated\<^sub>e (e2 @ [Return\<^sub>e]) \<Longrightarrow>
+    properly_terminated\<^sub>e (e1 @ PushEnv\<^sub>e # e2 @ [PopEnv\<^sub>e, Return\<^sub>e])"
+  by (induction e1 rule: properly_terminated\<^sub>e.induct) simp_all
 
-lemma [simp]: "assembly_mapb cd = assembly_map cd"
-  by rule simp
+lemma [simp]: "properly_terminated\<^sub>e (encode e)"
+  by (induction e) (simp_all add: encode_def)
 
-lemma alg_compile3_simp [simp]: "alg_compile3 cd = disassemble (assemble_code cd)"
-  by (simp_all add: alg_compile3_def assemble_code_def)
+theorem tc_success: "compile e = Some (cd, t) \<Longrightarrow> \<exists>e\<^sub>t. (Map.empty \<turnstile>\<^sub>t e\<^sub>t : t) \<and> erase e\<^sub>t = e \<and>
+  (\<exists>v. value\<^sub>s v \<and> e \<Down>\<^sub>s v \<and> (\<exists>\<Sigma>. final_state \<Sigma> \<and> iter (\<tturnstile> cd \<leadsto>\<^sub>m) (initial_state cd) \<Sigma> \<and> 
+    print_mach_state t \<Sigma> = print_nexpr v))"
+proof -
+  assume C: "compile e = Some (cd, t)"
+  then obtain e\<^sub>t where T: "typecheck e = Some (e\<^sub>t, t)" by (auto split: option.splits prod.splits)
+  hence TN: "(Map.empty \<turnstile>\<^sub>t e\<^sub>t : t) \<and> e = erase e\<^sub>t" by simp
+  then obtain v\<^sub>t where ET: "e\<^sub>t \<Down>\<^sub>s v\<^sub>t" by fastforce
+  with TN have VT: "value\<^sub>s v\<^sub>t \<and> Map.empty \<turnstile>\<^sub>t v\<^sub>t : t" by simp
+  hence VN: "value\<^sub>s (erase v\<^sub>t)" by simp
+  from ET have EN: "erase e\<^sub>t \<Down>\<^sub>s erase v\<^sub>t" by simp
+  from TN have TD: "[] \<turnstile>\<^sub>d unname e\<^sub>t : t" by simp
+  from ET TN have ED: "unname e\<^sub>t \<Down>\<^sub>d unname v\<^sub>t" by fastforce
+  hence VD: "value\<^sub>d (unname v\<^sub>t)" by simp
+  from ED have "iter (\<leadsto>\<^sub>d) (unname e\<^sub>t) (unname v\<^sub>t)" by (metis correct\<^sub>d\<^sub>b)
+  with ED EN TD have ES: "iter (\<leadsto>\<^sub>k) (S\<^sub>k False [FReturn\<^sub>k] (unname e\<^sub>t)) (S\<^sub>k True [] (unname v\<^sub>t))" 
+    by simp
+  from TD have TC: "SE\<^sub>c [FReturn\<^sub>c []] [] (unname e\<^sub>t) :\<^sub>c t" 
+    by (metisx tcc_state_ev tc\<^sub>c_nil tcc_snil tcc_scons_ret latest_environment.simps(4))
+  with ES VD EN obtain c where EC: "iter (\<leadsto>\<^sub>c) (SE\<^sub>c [FReturn\<^sub>c []] [] (unname e\<^sub>t)) (SC\<^sub>c [] c) \<and> 
+    declosure c = unname v\<^sub>t" by fastforce
+  from TC EC have "iter (\<leadsto>\<^sub>e) (encode_state (SE\<^sub>c [FReturn\<^sub>c []] [] (unname e\<^sub>t))) 
+    (encode_state (SC\<^sub>c [] c))" by (metis correct\<^sub>e_iter)
+  hence "iter (\<leadsto>\<^sub>e) (S\<^sub>e [] [([], encode (unname e\<^sub>t))]) (S\<^sub>e [encode_closure c] [])" 
+    by (simp add: encode_def)
+  moreover have "complete_lams_state (S\<^sub>e [] [([], encode (unname e\<^sub>t))])" by simp
+  ultimately have "iter (\<leadsto>\<^sub>e) (tco_state (S\<^sub>e [] [([], encode (unname e\<^sub>t))])) 
+    (tco_state (S\<^sub>e [encode_closure c] []))" by (metis correctness\<^sub>t\<^sub>c\<^sub>o_iter)
+  hence ET: "iter (\<leadsto>\<^sub>e) (S\<^sub>e [] [([], tco_code (encode (unname e\<^sub>t)))]) 
+    (S\<^sub>e [tco_val (encode_closure c)] [])" by (simp add: encode_def)
+  let ?cd = "(flatten_code \<circ> tco_code \<circ> encode \<circ> unname) e\<^sub>t"
+  have UB: "unflatten_state ?cd (S\<^sub>b [] [([], length ?cd)]) = 
+    S\<^sub>e [] [([], tco_code (encode (unname e\<^sub>t)))]" by simp
+  have "orderly_state ?cd (S\<^sub>b [] [([], length ?cd)])" by simp
+  with ET UB obtain v\<^sub>b where EB: "iter (\<tturnstile> ?cd \<leadsto>\<^sub>b) (S\<^sub>b [] [([], length ?cd)]) (S\<^sub>b [v\<^sub>b] []) \<and> 
+    tco_val (encode_closure c) = unflatten_closure ?cd v\<^sub>b" by (metis eval\<^sub>b_end)
+  then obtain \<Sigma>\<^sub>h' where EH: "iter (\<tturnstile> ?cd \<leadsto>\<^sub>h) (S\<^sub>h hempty [] [([], length ?cd)]) \<Sigma>\<^sub>h' \<and> 
+    S\<^sub>b [v\<^sub>b] [] = unheap \<Sigma>\<^sub>h'" by fastforce
+  then obtain h\<^sub>h v\<^sub>h where SH: "\<Sigma>\<^sub>h' = S\<^sub>h h\<^sub>h [v\<^sub>h] [] \<and> v\<^sub>b = unheap_closure h\<^sub>h v\<^sub>h" 
+    using unheap_to_empty by blast
+  have S\<^sub>h: "heap_structured (S\<^sub>h hempty [] [([], length ?cd)])" by simp
+  have S\<^sub>v: "unchain_state (S\<^sub>v hempty hempty [] [(0, length ?cd)]) = 
+    S\<^sub>h hempty [] [([], length ?cd)]" by simp
+  with EH SH obtain \<Sigma>\<^sub>c\<^sub>e' where ECE: "iter (\<tturnstile> ?cd \<leadsto>\<^sub>v) 
+    (S\<^sub>v hempty hempty [] [(0, length ?cd)]) \<Sigma>\<^sub>c\<^sub>e' \<and> S\<^sub>h h\<^sub>h [v\<^sub>h] [] = unchain_state \<Sigma>\<^sub>c\<^sub>e'" by fastforce
+  then obtain h\<^sub>c\<^sub>e env\<^sub>h where VCE: "\<Sigma>\<^sub>c\<^sub>e' = S\<^sub>v h\<^sub>c\<^sub>e env\<^sub>h [v\<^sub>h] [] \<and> h\<^sub>h = unchain_heap h\<^sub>c\<^sub>e env\<^sub>h" 
+    by (metis unchain_state_reverse map_is_Nil_conv)
+  let ?nmem = "\<lambda>x. undefined"
+  have CS: "chained_state (S\<^sub>v hempty hempty [] [(0, length ?cd)])" by simp
+  with ECE VCE have "iter (\<tturnstile> ?cd \<leadsto>\<^sub>f) (flatten (S\<^sub>v hempty hempty [] [(0, length ?cd)]))
+    (flatten (S\<^sub>v h\<^sub>c\<^sub>e env\<^sub>h [v\<^sub>h] []))" by (metis correct\<^sub>f_iter)
+  hence EF: "iter (\<tturnstile> ?cd \<leadsto>\<^sub>f) (S\<^sub>f (H ?nmem 0) (H ?nmem 0) [] [length ?cd, 0])
+     (S\<^sub>f (flatten_values h\<^sub>c\<^sub>e) (flatten_environment env\<^sub>h) [2 * v\<^sub>h] [])" by (simp add: hempty_def)
+  with ECE CS have "chained_state \<Sigma>\<^sub>c\<^sub>e'" by (metis preserve_chained)
+  with VCE have VH: "hcontains h\<^sub>c\<^sub>e v\<^sub>h" by simp
+  with EF have "\<exists>\<Sigma>\<^sub>u'. 
+    iter (\<tturnstile> ?cd \<leadsto>\<^sub>r) (S\<^sub>r ?nmem 0 ?nmem 0 ?nmem 0 (?nmem(0 := 0, 1 := 0)) 2 (length ?cd)) \<Sigma>\<^sub>u' \<and>
+      S\<^sub>f (flatten_values h\<^sub>c\<^sub>e) (flatten_environment env\<^sub>h) [2 * v\<^sub>h] [] = restructure \<Sigma>\<^sub>u'" by simp_all
+  then obtain \<Sigma>\<^sub>u' where EU:
+    "iter (\<tturnstile> ?cd \<leadsto>\<^sub>r) (S\<^sub>r ?nmem 0 ?nmem 0 ?nmem 0 (?nmem(0 := 0, 1 := 0)) 2 (length ?cd)) \<Sigma>\<^sub>u' \<and> 
+      S\<^sub>f (flatten_values h\<^sub>c\<^sub>e) (flatten_environment env\<^sub>h) [2 * v\<^sub>h] [] = restructure \<Sigma>\<^sub>u'" by blast
+  moreover then obtain h\<^sub>u hp\<^sub>u e\<^sub>u ep\<^sub>u vs\<^sub>u vp\<^sub>u sh\<^sub>u where VU:
+    "\<Sigma>\<^sub>u' = S\<^sub>r h\<^sub>u hp\<^sub>u e\<^sub>u ep\<^sub>u vs\<^sub>u vp\<^sub>u sh\<^sub>u 0 0 \<and> flatten_values h\<^sub>c\<^sub>e = H h\<^sub>u hp\<^sub>u \<and> 
+      flatten_environment env\<^sub>h = H e\<^sub>u ep\<^sub>u \<and> listify_heap vs\<^sub>u vp\<^sub>u = 2 * v\<^sub>h # []" by auto
+  moreover hence VSU: "vs\<^sub>u 0 = 2 * v\<^sub>h \<and> vp\<^sub>u = 1" by auto
+  ultimately have "iter (\<tturnstile> ?cd \<leadsto>\<^sub>r) (S\<^sub>r ?nmem 0 ?nmem 0 ?nmem 0 (?nmem(0 := 0, 1 := 0)) 2 
+    (length ?cd)) (S\<^sub>r h\<^sub>u hp\<^sub>u e\<^sub>u ep\<^sub>u vs\<^sub>u 1 sh\<^sub>u 0 0)" by simp
+  hence EU: "iter (\<tturnstile> ?cd \<leadsto>\<^sub>r) (S\<^sub>r ?nmem 0 ?nmem 0 ?nmem 0 (?nmem(0 := 0, 1 := 0)) 2 (length ?cd)) 
+    (S\<^sub>r h\<^sub>u hp\<^sub>u e\<^sub>u ep\<^sub>u vs\<^sub>u 1 sh\<^sub>u 0 0)" by simp
+  let ?cd' = "assemble_code ?cd"
+  let ?mp = "assembly_map ?cd"
+  let ?mem = "(case_prod (case_memseg (assm_hp ?cd ?nmem 0) (assemble_env ?nmem 0)
+    (assemble_vals ?nmem 0) (assm_stk ?cd (?nmem(0 := 0, 1 := 0)) 2) undefined))"
+  let ?mem' = "case_prod (case_memseg (assm_hp ?cd h\<^sub>u hp\<^sub>u) (assemble_env e\<^sub>u ep\<^sub>u) (assemble_vals vs\<^sub>u 1) 
+    (assm_stk ?cd sh\<^sub>u 0) undefined)"
+  let ?rs = "case_memseg (Hp, 0) (Env, 0) (Vals, 0) (Stk, 2) (Acc, 0)"
+  let ?rs' = "case_memseg (Hp, hp\<^sub>u) (Env, ep\<^sub>u) (Vals, Suc 0) (Stk, 0) (Acc, 0)"
+  have "assembleable (S\<^sub>r ?nmem 0 ?nmem 0 ?nmem 0 (?nmem(0 := 0, 1 := 0)) 2 (length ?cd)) ?cd" 
+    by simp
+  with EU have "iter (\<tturnstile> ?cd' \<leadsto>\<^sub>a) 
+    (assemble_state ?mp (S\<^sub>r ?nmem 0 ?nmem 0 ?nmem 0 (?nmem(0 := 0, 1 := 0)) 2 (length ?cd))) 
+      (assemble_state ?mp (S\<^sub>r h\<^sub>u hp\<^sub>u e\<^sub>u ep\<^sub>u vs\<^sub>u 1 sh\<^sub>u 0 0))" by (metis correct\<^sub>a_iter)
+  hence "iter (\<tturnstile> ?cd' \<leadsto>\<^sub>a) (S\<^sub>a ?mem ?rs (length ?cd')) (S\<^sub>a ?mem' ?rs' 0)" by simp
+  hence "iter (\<tturnstile> disassemble ?cd' \<leadsto>\<^sub>m) (disassemble_state (S\<^sub>a ?mem ?rs (length ?cd'))) 
+    (disassemble_state (S\<^sub>a ?mem' ?rs' 0))" by (metis correctm_iter)
+  hence "iter (\<tturnstile> disassemble ?cd' \<leadsto>\<^sub>m) (MS (case_reg 0 1 2 11 0)
+    (unmap_mem (case_prod (case_memseg (\<lambda>x. (Acc, 0)) (\<lambda>x. (Acc, 0)) (\<lambda>x. (Acc, 0)) 
+      ((\<lambda>x. (Acc, 0))(0 := (Acc, 0), Suc 0 := (Env, 0))) undefined))) (length ?cd')) 
+        (MS (case_reg (4 * hp\<^sub>u) (Suc (4 * ep\<^sub>u)) 6 3 0) (unmap_mem ?mem') 0)" 
+    by simp
+  with C T have EM: "iter (\<tturnstile> cd \<leadsto>\<^sub>m) (MS (case_reg 0 1 2 11 0) ((\<lambda>x. 0)(7 := 1)) 
+    (length cd)) (MS (case_reg (4 * hp\<^sub>u) (Suc (4 * ep\<^sub>u)) 6 3 0) (unmap_mem ?mem') 0)" by auto
+  from EC VT have "print_closure c = print_nexpr (erase v\<^sub>t)" by simp
+  moreover from EB have "print_bclosure v\<^sub>b = print_eclosure (tco_val (encode_closure c))" by simp
+  ultimately have "print_bclosure v\<^sub>b = print_nexpr (erase v\<^sub>t)" by simp
+  with SH have "print_hclosure (hlookup h\<^sub>h v\<^sub>h) = print_nexpr (erase v\<^sub>t)" by simp
+  with VCE VH have PH: "print_ceclosure (hlookup h\<^sub>c\<^sub>e v\<^sub>h) = print_nexpr (erase v\<^sub>t)" 
+    by (metis print_ce)
+  with VT have TT: "top_level t = closure_ty (hlookup h\<^sub>c\<^sub>e v\<^sub>h)" by auto
+  with VH PH have "print_ceclosure (get_closure t (flatten_values h\<^sub>c\<^sub>e) (2 * v\<^sub>h)) = 
+    print_nexpr (erase v\<^sub>t)" by simp
+  with VU VSU have PU: "print_uval t (snd \<circ> h\<^sub>u) (vs\<^sub>u 0) = print_nexpr (erase v\<^sub>t)" by (metis print_u)
+  from VH VU VSU have SH: "Suc (vs\<^sub>u 0) < hp\<^sub>u" by (metis flatten_lt_3)
+  from VSU have V3: "even (vs\<^sub>u 0)" by simp
+  from VU VSU VH TT have "hp_tc t h\<^sub>u (vs\<^sub>u 0)" by simp
+  with SH V3 PU have PU2: "print_uval t (pseudoreg_map \<circ> assm_hp ?cd h\<^sub>u hp\<^sub>u) (vs\<^sub>u 0) = 
+    print_nexpr (erase v\<^sub>t)" by (metis print_a)
+  have "unmap_mem' (unmap_mem ?mem' 2) = (Hp, vs\<^sub>u 0)"
+    by (auto simp add: numeral_def split: prod.splits memseg.splits) 
+       (simp add: assemble_vals_def unmap_mem_def)
+  hence "print_mach_state t (MS (case_reg (4 * hp\<^sub>u) (Suc (4 * ep\<^sub>u)) 6 3 0) 
+    (unmap_mem ?mem') 0) = print_uval t (unmap_mem ?mem') (4 * vs\<^sub>u 0)" by simp
+  with PU2 have PM: "print_mach_state t (MS (case_reg (4 * hp\<^sub>u) (Suc (4 * ep\<^sub>u)) 6 3 0) 
+    (unmap_mem ?mem') 0) = print_nexpr (erase v\<^sub>t)" by (metis print_q)
+  have "final_state (MS (case_reg (4 * hp\<^sub>u) (Suc (4 * ep\<^sub>u)) 6 3 0) (unmap_mem ?mem') 0)" by simp
+  with VN TN EN EM PM show ?thesis by blast
+qed
 
-lemma [simp]: "collect_constraints \<Gamma> vs e = snd (typecheck' \<Gamma> vs e)"
-  by (induction e arbitrary: \<Gamma> vs) (simp_all add: Let_def split: option.splits prod.splits)
+text \<open>We have now proven the correctness of our compiler; but, as Donald Knuth once said, "beware of 
+bugs in the above code; I have only proved it correct, not tried it." [8] So we will leave off with 
+some small example programs, to show what it looks like in practice.\<close>
 
-lemma alg_compile_simp [simp]: "alg_compile = compile"
-  by rule (simp add: alg_compile_def encode_def flatten_code_def unname_def split: prod.splits option.splits)
+abbreviation churchTrue :: "unit expr\<^sub>s" 
+  where "churchTrue \<equiv> Lam\<^sub>s (V ''x'') () (Lam\<^sub>s (V ''y'') () (Var\<^sub>s (V ''x'')))"
+
+abbreviation churchFalse :: "unit expr\<^sub>s" 
+  where "churchFalse \<equiv> Lam\<^sub>s (V ''x'') () (Lam\<^sub>s (V ''y'') () (Var\<^sub>s (V ''y'')))"
+
+abbreviation churchIf :: "unit expr\<^sub>s" 
+  where "churchIf \<equiv> 
+    Lam\<^sub>s (V ''b'') () (Lam\<^sub>s (V ''x'') () (Lam\<^sub>s (V ''y'') () 
+      (App\<^sub>s (App\<^sub>s (Var\<^sub>s (V ''b'')) (Var\<^sub>s (V ''x''))) (Var\<^sub>s (V ''y'')))))"
+
+value "compile (Let\<^sub>s (V ''churchTrue'') churchTrue (Let\<^sub>s (V ''churchIf'') churchIf (
+       App\<^sub>s (App\<^sub>s (App\<^sub>s (Var\<^sub>s (V ''churchIf'')) (Var\<^sub>s (V ''churchTrue''))) (Const\<^sub>s 3)) (Const\<^sub>s 5))))"
 
 end
